lean/love02_backward_proofs_exercise_sheet.lean
@@ -1,15 +1,18 @@
 import .love02_backward_proofs_demo
 
 
-/-! # LoVe Exercise 2: Backward Proofs -/
+/- # LoVe Exercise 2: Backward Proofs -/
 
 
 set_option pp.beta true
+set_option pp.generalized_field_notation false
 
 namespace LoVe
 
+namespace backward_proofs
 
-/-! ## Question 1: Connectives and Quantifiers
+
+/- ## Question 1: Connectives and Quantifiers
 
 1.1. Carry out the following proofs using basic tactics.
 
@@ -32,7 +35,7 @@ lemma proj_1st (a : Prop) :
   a → a → a :=
 sorry
 
-/-! Please give a different answer than for `proj_1st`: -/
+/- Please give a different answer than for `proj_1st`: -/
 
 lemma proj_2nd (a : Prop) :
   a → a → a :=
@@ -42,13 +45,13 @@ lemma some_nonsense (a b c : Prop) :
   (a → b → c) → a → (a → c) → b → c :=
 sorry
 
-/-! 1.2. Prove the contraposition rule using basic tactics. -/
+/- 1.2. Prove the contraposition rule using basic tactics. -/
 
 lemma contrapositive (a b : Prop) :
   (a → b) → ¬ b → ¬ a :=
 sorry
 
-/-! 1.3. Prove the distributivity of `∀` over `∧` using basic tactics.
+/- 1.3. Prove the distributivity of `∀` over `∧` using basic tactics.
 
 Hint: This exercise is tricky, especially the right-to-left direction. Some
 forward reasoning, like in the proof of `and_swap₂` in the lecture, might be
@@ -59,7 +62,7 @@ lemma forall_and {α : Type} (p q : α → Prop) :
 sorry
 
 
-/-! ## Question 2: Natural Numbers
+/- ## Question 2: Natural Numbers
 
 2.1. Prove the following recursive equations on the first argument of the
 `mul` operator defined in lecture 1. -/
@@ -74,18 +77,18 @@ lemma mul_succ (m n : ℕ) :
   mul (nat.succ m) n = add (mul m n) n :=
 sorry
 
-/-! 2.2. Prove commutativity and associativity of multiplication using the
-`induction` tactic. Choose the induction variable carefully. -/
+/- 2.2. Prove commutativity and associativity of multiplication using the
+`induction'` tactic. Choose the induction variable carefully. -/
 
 lemma mul_comm (m n : ℕ) :
   mul m n = mul n m :=
 sorry
 
 lemma mul_assoc (l m n : ℕ) :
-  mul (mul l m) n = mul l (mul m n) := :=
+  mul (mul l m) n = mul l (mul m n) :=
 sorry
 
-/-! 2.3. Prove the symmetric variant of `mul_add` using `rewrite`. To apply
+/- 2.3. Prove the symmetric variant of `mul_add` using `rw`. To apply
 commutativity at a specific position, instantiate the rule by passing some
 arguments (e.g., `mul_comm _ l`). -/
 
@@ -94,7 +97,7 @@ lemma add_mul (l m n : ℕ) :
 sorry
 
 
-/-! ## Question 3 (**optional**): Intuitionistic Logic
+/- ## Question 3 (**optional**): Intuitionistic Logic
 
 Intuitionistic logic is extended to classical logic by assuming a classical
 axiom. There are several possibilities for the choice of axiom. In this
@@ -110,26 +113,26 @@ def peirce :=
 def double_negation :=
 ∀a : Prop, (¬¬ a) → a
 
-/-! For the proofs below, please avoid using lemmas from Lean's `classical`
+/- For the proofs below, please avoid using lemmas from Lean's `classical`
 namespace, because this would defeat the purpose of the exercise.
 
 3.1 (**optional**). Prove the following implication using tactics.
 
 Hint: You will need `or.elim` and `false.elim`. You can use
-`simp [excluded_middle, peirce]` to unfold the definitions of `excluded_middle`
-and `peirce`. -/
+`rw excluded_middle` to unfold the definition of `excluded_middle`,
+and similarly for `peirce`. -/
 
 lemma peirce_of_em :
   excluded_middle → peirce :=
 sorry
 
-/-! 3.2 (**optional**). Prove the following implication using tactics. -/
+/- 3.2 (**optional**). Prove the following implication using tactics. -/
 
 lemma dn_of_peirce :
   peirce → double_negation :=
 sorry
 
-/-! We leave the missing implication for the homework: -/
+/- We leave the missing implication for the homework: -/
 
 namespace sorry_lemmas
 
@@ -138,5 +141,7 @@ lemma em_of_dn :
 sorry
 
 end sorry_lemmas
+
+end backward_proofs
 
 end LoVe
