lean/love03_forward_proofs_exercise_sheet.lean
@@ -1,15 +1,16 @@
 import .lovelib
 
 
-/-! # LoVe Exercise 3: Forward Proofs -/
+/- # LoVe Exercise 3: Forward Proofs -/
 
 
 set_option pp.beta true
+set_option pp.generalized_field_notation false
 
 namespace LoVe
 
 
-/-! ## Question 1: Connectives and Quantifiers
+/- ## Question 1: Connectives and Quantifiers
 
 1.1. Supply structured proofs of the following lemmas. -/
 
@@ -29,7 +30,7 @@ lemma proj_1st (a : Prop) :
   a → a → a :=
 sorry
 
-/-! Please give a different answer than for `proj_1st`. -/
+/- Please give a different answer than for `proj_1st`. -/
 
 lemma proj_2nd (a : Prop) :
   a → a → a :=
@@ -39,19 +40,19 @@ lemma some_nonsense (a b c : Prop) :
   (a → b → c) → a → (a → c) → b → c :=
 sorry
 
-/-! 1.2. Supply a structured proof of the contraposition rule. -/
+/- 1.2. Supply a structured proof of the contraposition rule. -/
 
 lemma contrapositive (a b : Prop) :
   (a → b) → ¬ b → ¬ a :=
 sorry
 
-/-! 1.3. Supply a structured proof of the distributivity of `∀` over `∧`. -/
+/- 1.3. Supply a structured proof of the distributivity of `∀` over `∧`. -/
 
 lemma forall_and {α : Type} (p q : α → Prop) :
   (∀x, p x ∧ q x) ↔ (∀x, p x) ∧ (∀x, q x) :=
 sorry
 
-/-! 1.4. Reuse, if possible, the lemma `forall_and` you proved above to prove
+/- 1.4. Reuse, if possible, the lemma `forall_and` you proved above to prove
 the following instance of the lemma. -/
 
 lemma forall_and_inst {α : Type} (r s : α → α → Prop) :
@@ -59,7 +60,7 @@ lemma forall_and_inst {α : Type} (r s : α → α → Prop) :
 sorry
 
 
-/-! ## Question 2: Chain of Equalities
+/- ## Question 2: Chain of Equalities
 
 2.1. Write the following proof using `calc`.
 
@@ -76,14 +77,14 @@ lemma binomial_square (a b : ℕ) :
   (a + b) * (a + b) = a * a + 2 * a * b + b * b :=
 sorry
 
-/-! 2.2. Prove the same argument again, this time as a structured proof. Try to
+/- 2.2. Prove the same argument again, this time as a structured proof. Try to
 reuse as much of the above proof idea as possible. -/
 
 lemma binomial_square₂ (a b : ℕ) :
   (a + b) * (a + b) = a * a + 2 * a * b + b * b :=
 sorry
 
-/-! 2.3. Prove the same lemma again, this time using tactics. -/
+/- 2.3. Prove the same lemma again, this time using tactics. -/
 
 lemma binomial_square₃ (a b : ℕ) :
   (a + b) * (a + b) = a * a + 2 * a * b + b * b :=
@@ -92,7 +93,7 @@ begin
 end
 
 
-/-! ## Question 3 (**optional**): One-Point Rules
+/- ## Question 3 (**optional**): One-Point Rules
 
 3.1 (**optional**). Prove that the following wrong formulation of the one-point
 rule for `∀` is inconsistent, using a structured proof. -/
@@ -104,7 +105,7 @@ lemma proof_of_false :
   false :=
 sorry
 
-/-! 3.2 (**optional**). Prove that the following wrong formulation of the
+/- 3.2 (**optional**). Prove that the following wrong formulation of the
 one-point rule for `∃` is inconsistent, using a tactical or structured proof. -/
 
 axiom exists.one_point_wrong {α : Type} {t : α} {p : α → Prop} :
