lean/love05_inductive_predicates_exercise_sheet.lean
@@ -1,38 +1,39 @@
 import .love05_inductive_predicates_demo
 
 
-/-! # LoVe Exercise 5: Inductive Predicates -/
+/- # LoVe Exercise 5: Inductive Predicates -/
 
 
 set_option pp.beta true
+set_option pp.generalized_field_notation false
 
 namespace LoVe
 
 
-/-! ## Question 1: Even and Odd
+/- ## Question 1: Even and Odd
 
 The `even` predicate is true for even numbers and false for odd numbers. -/
 
 #check even
 
-/-! We define `odd` as the negation of `even`: -/
+/- We define `odd` as the negation of `even`: -/
 
 def odd (n : ℕ) : Prop :=
   ¬ even n
 
-/-! 1.1. Prove that 1 is odd and register this fact as a simp rule.
+/- 1.1. Prove that 1 is odd and register this fact as a simp rule.
 
-Hint: `cases` is useful to reason about hypotheses of the form `even …`. -/
+Hint: `cases'` is useful to reason about hypotheses of the form `even …`. -/
 
 @[simp] lemma odd_1 :
   odd 1 :=
 sorry
 
-/-! 1.2. Prove that 3, 5, and 7 are odd. -/
+/- 1.2. Prove that 3, 5, and 7 are odd. -/
 
 -- enter your answer here
 
-/-! 1.3. Complete the following proof by structural induction. -/
+/- 1.3. Complete the following proof by structural induction. -/
 
 lemma even_two_times :
   ∀m : ℕ, even (2 * m)
@@ -40,24 +41,24 @@ lemma even_two_times :
 | (m + 1) :=
   sorry
 
-/-! 1.4. Complete the following proof by rule induction.
+/- 1.4. Complete the following proof by rule induction.
 
-Hint: You can use the `cases` tactic (or `match … with`) to destruct an
+Hint: You can use the `cases'` tactic (or `match … with`) to destruct an
 existential quantifier and extract the witness. -/
 
 lemma even_imp_exists_two_times :
   ∀n : ℕ, even n → ∃m, n = 2 * m :=
 begin
   intros n hen,
-  induction hen,
-  case even.zero {
+  induction' hen,
+  case zero {
     apply exists.intro 0,
     refl },
-  case even.add_two : k hek ih {
+  case add_two : k hek ih {
     sorry }
 end
 
-/-! 1.6. Using `even_two_times` and `even_imp_exists_two_times`, prove the
+/- 1.6. Using `even_two_times` and `even_imp_exists_two_times`, prove the
 following equivalence. -/
 
 lemma even_iff_exists_two_times (n : ℕ) :
@@ -65,7 +66,7 @@ lemma even_iff_exists_two_times (n : ℕ) :
 sorry
 
 
-/-! ## Question 2: Binary Trees
+/- ## Question 2: Binary Trees
 
 2.1. Prove the converse of `is_full_mirror`. You may exploit already proved
 lemmas (e.g., `is_full_mirror`, `mirror_mirror`). -/
@@ -77,18 +78,18 @@ lemma mirror_is_full {α : Type} :
   ∀t : btree α, is_full (mirror t) → is_full t :=
 sorry
 
-/-! 2.2. Define a `map` function on binary trees, similar to `list.map`. -/
+/- 2.2. Define a `map` function on binary trees, similar to `list.map`. -/
 
 def btree.map {α β : Type} (f : α → β) : btree α → btree β
--- enter the missing cases here
+| _ := sorry   -- remove this dummy case and enter the missing cases
 
-/-! 2.3. Prove the following lemma by case distinction. -/
+/- 2.3. Prove the following lemma by case distinction. -/
 
 lemma btree.map_eq_empty_iff {α β : Type} (f : α → β) :
   ∀t : btree α, btree.map f t = btree.empty ↔ t = btree.empty :=
 sorry
 
-/-! 2.4. Prove the following lemma by rule induction. -/
+/- 2.4. Prove the following lemma by rule induction. -/
 
 lemma btree.map_mirror {α β : Type} (f : α → β) :
   ∀t : btree α, is_full t → is_full (btree.map f t) :=
