lean/love09_hoare_logic_exercise_sheet.lean
@@ -1,15 +1,16 @@
 import .love09_hoare_logic_demo
 
 
-/-! # LoVe Exercise 9: Hoare Logic -/
+/- # LoVe Exercise 9: Hoare Logic -/
 
 
 set_option pp.beta true
+set_option pp.generalized_field_notation false
 
 namespace LoVe
 
 
-/-! ## Question 1: Program Verification
+/- ## Question 1: Program Verification
 
 The following WHILE program is intended to compute the Gaussian sum up to `n`,
 leaving the result in `r`. -/
@@ -20,13 +21,13 @@ stmt.while (λs, s "n" ≠ 0)
   (stmt.assign "r" (λs, s "r" + s "n") ;;
    stmt.assign "n" (λs, s "n" - 1))
 
-/-! The summation function: -/
+/- The summation function: -/
 
 def sum_upto : ℕ → ℕ
 | 0       := 0
 | (n + 1) := n + 1 + sum_upto n
 
-/-! 1.1. Prove the correctness of `GAUSS` using `vcg`. The main challenge is to
+/- 1.1. Prove the correctness of `GAUSS` using `vcg`. The main challenge is to
 figure out which invariant to use for the while loop. The invariant should
 capture both the work that has been done already (the intermediate result) and
 the work that remains to be done. -/
@@ -35,7 +36,7 @@ lemma GAUSS_correct (n₀ : ℕ) :
   {* λs, s "n" = n₀ *} GAUSS {* λs, s "r" = sum_upto n₀ *} :=
 sorry
 
-/-! 1.2. The following WHILE program is intended to compute the product of `n`
+/- 1.2. The following WHILE program is intended to compute the product of `n`
 and `m`, leaving the result in `r`. Prove its correctness using `vcg`.
 
 Hint: If a variable `x` does not change in a program, it might be useful to
@@ -52,7 +53,7 @@ lemma MUL_correct (n₀ m₀ : ℕ) :
 sorry
 
 
-/-! ## Question 2: Hoare Triples for Total Correctness -/
+/- ## Question 2: Hoare Triples for Total Correctness -/
 
 def total_hoare (P : state → Prop) (S : stmt) (Q : state → Prop) : Prop :=
 ∀s, P s → ∃t, (S, s) ⟹ t ∧ Q t
@@ -62,32 +63,32 @@ total_hoare P S Q
 
 namespace total_hoare
 
-/-! 2.1. Prove the consequence rule. -/
+/- 2.1. Prove the consequence rule. -/
 
 lemma consequence {P P' Q Q' : state → Prop} {S}
     (hS : [* P *] S [* Q *]) (hP : ∀s, P' s → P s) (hQ : ∀s, Q s → Q' s) :
   [* P' *] S [* Q' *] :=
 sorry
 
-/-! 2.2. Prove the rule for `skip`. -/
+/- 2.2. Prove the rule for `skip`. -/
 
 lemma skip_intro {P} :
   [* P *] stmt.skip [* P *] :=
 sorry
 
-/-! 2.3. Prove the rule for `assign`. -/
+/- 2.3. Prove the rule for `assign`. -/
 
 lemma assign_intro {P : state → Prop} {x} {a : state → ℕ} :
   [* λs, P (s{x ↦ a s}) *] stmt.assign x a [* P *] :=
 sorry
 
-/-! 2.4. Prove the rule for `seq`. -/
+/- 2.4. Prove the rule for `seq`. -/
 
 lemma seq_intro {P Q R S T} (hS : [* P *] S [* Q *]) (hT : [* Q *] T [* R *]) :
   [* P *] S ;; T [* R *] :=
 sorry
 
-/-! 2.5. Complete the proof of the rule for `ite`.
+/- 2.5. Complete the proof of the rule for `ite`.
 
 Hint: This requires a case distinction on the truth value of `b s`. -/
 
@@ -97,30 +98,30 @@ lemma ite_intro {b P Q : state → Prop} {S T}
   [* P *] stmt.ite b S T [* Q *] :=
 sorry
 
-/-! 2.6 (**optional**). Try to prove the rule for `while`.
+/- 2.6 (**optional**). Try to prove the rule for `while`.
 
 The rule is parameterized by a loop invariant `I` and by a variant `V` that
 decreases with each iteration of the loop body.
 
 Before we prove the desired lemma, we introduce an auxiliary lemma. Its proof
-requires well-founded induction. When using `while_intro.aux` as induction
+requires well-founded induction. When using `while_var_intro_aux` as induction
 hypothesis we recommend to do it directly after proving that the argument is
 less than `v₀`:
 
     have ih : ∃u, (stmt.while b S, t) ⟹ u ∧ I u ∧ ¬ b u :=
       have V t < v₀ :=
         …,
-      while_intro.aux (V t) …,
+      while_var_intro_aux (V t) …,
 
 Similarly to `ite`, the proof requires a case distinction on `b s ∨ ¬ b s`. -/
 
-lemma while_intro.aux {b : state → Prop} (I : state → Prop) (V : state → ℕ) {S}
-  (h_inv : ∀v₀, [* λs, I s ∧ b s ∧ V s = v₀ *] S [* λs, I s ∧ V s < v₀ *]) :
+lemma while_var_intro_aux {b : state → Prop} (I : state → Prop) (V : state → ℕ)
+  {S} (h_inv : ∀v₀, [* λs, I s ∧ b s ∧ V s = v₀ *] S [* λs, I s ∧ V s < v₀ *]) :
   ∀v₀ s, V s = v₀ → I s → ∃t, (stmt.while b S, s) ⟹ t ∧ I t ∧ ¬ b t
 | v₀ s V_eq hs :=
 sorry
 
-lemma while_intro {b : state → Prop} (I : state → Prop) (V : state → ℕ) {S}
+lemma while_var_intro {b : state → Prop} (I : state → Prop) (V : state → ℕ) {S}
   (hinv : ∀v₀, [* λs, I s ∧ b s ∧ V s = v₀ *] S [* λs, I s ∧ V s < v₀ *]) :
   [* I *] stmt.while b S [* λs, I s ∧ ¬ b s *] :=
 sorry
