lean/love11_logical_foundations_of_mathematics_exercise_sheet.lean
@@ -1,21 +1,22 @@
 import .love11_logical_foundations_of_mathematics_demo
 
 
-/-! # LoVe Exercise 11: Logical Foundations of Mathematics -/
+/- # LoVe Exercise 11: Logical Foundations of Mathematics -/
 
 
 set_option pp.beta true
+set_option pp.generalized_field_notation false
 
 namespace LoVe
 
 
-/-! ## Question 1: Vectors as Subtypes
+/- ## Question 1: Vectors as Subtypes
 
 Recall the definition of vectors from the demo: -/
 
 #check vector
 
-/-! The following function adds two lists of integers elementwise. If one
+/- The following function adds two lists of integers elementwise. If one
 function is longer than the other, the tail of the longer function is
 truncated. -/
 
@@ -25,7 +26,7 @@ def list.add : list ℤ → list ℤ → list ℤ
 | []        (y :: ys) := []
 | (x :: xs) []        := []
 
-/-! 1.1. Show that if the lists have the same length, the resulting list also
+/- 1.1. Show that if the lists have the same length, the resulting list also
 has that length. -/
 
 lemma list.length_add :
@@ -40,13 +41,13 @@ lemma list.length_add :
 | (x :: xs) []        :=
   sorry
 
-/-! 1.2. Define componentwise addition on vectors using `list.add` and
-`length.length_add`. -/
+/- 1.2. Define componentwise addition on vectors using `list.add` and
+`list.length_add`. -/
 
 def vector.add {n : ℕ} : vector ℤ n → vector ℤ n → vector ℤ n :=
 sorry
 
-/-! 1.3. Show that `list.add` and `vector.add` are commutative. -/
+/- 1.3. Show that `list.add` and `vector.add` are commutative. -/
 
 lemma list.add.comm :
   ∀(xs : list ℤ) (ys : list ℤ), list.add xs ys = list.add ys xs :=
@@ -57,7 +58,7 @@ lemma vector.add.comm {n : ℕ} (x y : vector ℤ n) :
 sorry
 
 
-/-! ## Question 2: Integers as Quotients
+/- ## Question 2: Integers as Quotients
 
 Recall the construction of integers from the lecture, not to be confused with
 Lean's predefined type `int` (= `ℤ`): -/
@@ -66,12 +67,12 @@ Lean's predefined type `int` (= `ℤ`): -/
 #check int.rel_iff
 #check int
 
-/-! 2.1. Define negation on these integers. -/
+/- 2.1. Define negation on these integers. -/
 
 def int.neg : int → int :=
 sorry
 
-/-! 2.2. Prove the following lemmas about negation. -/
+/- 2.2. Prove the following lemmas about negation. -/
 
 lemma int.neg_eq (p n : ℕ) :
   int.neg ⟦(p, n)⟧ = ⟦(n, p)⟧ :=
