lean/love12_basic_mathematical_structures_exercise_sheet.lean
@@ -1,21 +1,22 @@
 import .love12_basic_mathematical_structures_demo
 
 
-/-! # LoVe Exercise 12: Basic Mathematical Structures -/
+/- # LoVe Exercise 12: Basic Mathematical Structures -/
 
 
 set_option pp.beta true
+set_option pp.generalized_field_notation false
 
 namespace LoVe
 
 
-/-! ## Question 1: Type Classes
+/- ## Question 1: Type Classes
 
 Recall the datatype `btree` we introduced earlier: -/
 
 #check btree
 
-/-! The following function takes two trees and attaches copies of the second
+/- The following function takes two trees and attaches copies of the second
 tree to each leaf of the first tree. -/
 
 def btree.graft {α : Type} : btree α → btree α → btree α
@@ -25,7 +26,7 @@ def btree.graft {α : Type} : btree α → btree α → btree α
 #reduce btree.graft (btree.node 1 btree.empty btree.empty)
   (btree.node 2 btree.empty btree.empty)
 
-/-! 1.1. Prove the following two lemmas by structural induction on `t`. -/
+/- 1.1. Prove the following two lemmas by structural induction on `t`. -/
 
 lemma btree.graft_assoc {α : Type} (t u v : btree α) :
   btree.graft (btree.graft t u) v = btree.graft t (btree.graft u v) :=
@@ -35,7 +36,7 @@ lemma btree.graft_empty {α : Type} (t : btree α) :
   btree.graft t btree.empty = t :=
 sorry
 
-/-! 1.2. Declare btree an instance of `add_monoid` using `graft` as addition
+/- 1.2. Declare btree an instance of `add_monoid` using `graft` as addition
 operator. -/
 
 #print add_monoid
@@ -43,12 +44,12 @@ operator. -/
 @[instance] def btree.add_monid {α : Type} : add_monoid (btree α) :=
 sorry
 
-/-! 1.3. Explain why `btree` with `graft` as addition cannot be declared an
+/- 1.3. Explain why `btree` with `graft` as addition cannot be declared an
 instance of `add_group`. -/
 
 #print add_group
 
-/-! 1.4 (**optional**). Prove the following lemma illustrating why `btree` with
+/- 1.4 (**optional**). Prove the following lemma illustrating why `btree` with
 `graft` as addition does not constitute an `add_group`. -/
 
 lemma btree.add_left_neg_counterexample :
@@ -56,7 +57,7 @@ lemma btree.add_left_neg_counterexample :
 sorry
 
 
-/-! ## Question 2: Multisets and Finsets
+/- ## Question 2: Multisets and Finsets
 
 Recall the following definitions from the lecture: -/
 
@@ -64,7 +65,7 @@ Recall the following definitions from the lecture: -/
 #check finset.elems
 #check list.elems
 
-/-! 2.1. Prove that the multiset of nodes does not change when mirroring a tree.
+/- 2.1. Prove that the multiset of nodes does not change when mirroring a tree.
 
 Hints:
 
@@ -76,14 +77,14 @@ lemma multiset.elems_mirror (t : btree ℕ) :
   multiset.elems (mirror t) = multiset.elems t :=
 sorry
 
-/-! 2.2. Prove that the finite set of nodes does not change when mirroring a
+/- 2.2. Prove that the finite set of nodes does not change when mirroring a
 tree. -/
 
 lemma finset.elems_mirror (t : btree ℕ) :
   finset.elems (mirror t) = finset.elems t :=
 sorry
 
-/-! 2.3. Show that this does not hold for the list of nodes by providing a
+/- 2.3. Show that this does not hold for the list of nodes by providing a
 tree `t` for which `nodes_list t ≠ nodes_list (mirror t)`.
 
 If you define a suitable counterexample, the proof below will succeed. -/
