lean/love13_rational_and_real_numbers_exercise_sheet.lean
@@ -2,15 +2,16 @@ import .love05_inductive_predicates_demo
 import .love13_rational_and_real_numbers_demo
 
 
-/-! # LoVe Exercise 13: Rational and Real Numbers -/
+/- # LoVe Exercise 13: Rational and Real Numbers -/
 
 
 set_option pp.beta true
+set_option pp.generalized_field_notation false
 
 namespace LoVe
 
 
-/-! ## Question 1: Rationals
+/- ## Question 1: Rationals
 
 1.1. Prove the following lemma.
 
@@ -23,7 +24,7 @@ lemma fraction.ext (a b : fraction) (hnum : fraction.num a = fraction.num b)
   a = b :=
 sorry
 
-/-! 1.2. Extending the `fraction.has_mul` instance from the lecture, declare
+/- 1.2. Extending the `fraction.has_mul` instance from the lecture, declare
 `fraction` as an instance of `semigroup`.
 
 Hint: Use the lemma `fraction.ext` above, and possibly `fraction.mul_num`, and
@@ -38,7 +39,7 @@ Hint: Use the lemma `fraction.ext` above, and possibly `fraction.mul_num`, and
     sorry,
   ..fraction.has_mul }
 
-/-! 1.3. Extending the `rat.has_mul` instance from the lecture, declare `rat` as
+/- 1.3. Extending the `rat.has_mul` instance from the lecture, declare `rat` as
 an instance of `semigroup`. -/
 
 @[instance] def rat.semigroup : semigroup rat :=
